spec/Correctness.ec
@@ -6,9 +6,37 @@ pragma Goals : printall.
 (* The preprocessed EasyCrypt is the same as the extracted EasyCrypt, but replaces calls to core_hash with calls
    to an operator H *)
 
-require import XMSS_IMPL.
-require import XMSS_IMPL_PP.
+require import AllCore IntDiv CoreMap List Distr.
+from Jasmin require import JModel.
 
-require import Address.
+require import Array32 Array68 Array96 Array128 Array136.
 
+require import XMSS_IMPL XMSS_IMPL_PP.
 
+op Hash_96 : W8.t Array32.t -> W8.t Array96.t -> W8.t Array32.t.
+op Hash_128 : W8.t Array32.t -> W8.t Array128.t -> W8.t Array32.t.
+op Hash_ptr : W8.t Array32.t -> W64.t -> W64.t -> W8.t Array32.t.
+
+(**********************************************************************************************************************)
+
+axiom hash_96 (out : W8.t Array32.t, in_0 : W8.t Array96.t) :   
+   hoare[M(Syscall).__core_hash_96 : arg = (out, in_0) ==> res = Hash_96 out in_0].   
+
+axiom hash__96 (out : W8.t Array32.t, in_0 : W8.t Array96.t) :   
+   hoare[M(Syscall)._core_hash_96 : arg = (out, in_0) ==> res = Hash_96 out in_0].   
+
+axiom hash_128 (out : W8.t Array32.t, in_0 : W8.t Array128.t) :   
+   hoare[M(Syscall).__core_hash_128 : arg = (out, in_0) ==> res = Hash_128 out in_0].   
+
+axiom hash__128 (out : W8.t Array32.t, in_0 : W8.t Array128.t) :   
+   hoare[M(Syscall)._core_hash_128 : arg = (out, in_0) ==> res = Hash_128 out in_0].   
+
+(**********************************************************************************************************************)
+
+lemma xmss_keypair_jazz_equiv (_pk : W8.t Array68.t, _sk : W8.t Array136.t) :
+equiv[M(Syscall).xmss_keypair_jazz ~ Mp(Syscall).xmss_keypair_jazz : true ==> ={res}].
+proof.
+proc.
+auto => />.
+admit.
+qed.
