spec/extraction/XMSS_IMPL.ec
@@ -877,19 +877,19 @@ module M(SC:Syscall_t) = {
     return (out);
   }
   
-  proc __core_hash_128 (out:W8.t Array32.t, in_0:W8.t Array128.t) : W8.t Array32.t = {
-    
-    
-    
-    out <@ __sha256_128 (out, in_0);
-    return (out);
-  }
-  
   proc __core_hash_96 (out:W8.t Array32.t, in_0:W8.t Array96.t) : W8.t Array32.t = {
     
     
     
     out <@ __sha256_96 (out, in_0);
+    return (out);
+  }
+  
+  proc __core_hash_128 (out:W8.t Array32.t, in_0:W8.t Array128.t) : W8.t Array32.t = {
+    
+    
+    
+    out <@ __sha256_128 (out, in_0);
     return (out);
   }
   
@@ -950,6 +950,17 @@ module M(SC:Syscall_t) = {
     return (out);
   }
   
+  proc __u32_to_bytes (out:W8.t Array4.t, in_0:W32.t) : W8.t Array4.t = {
+    
+    
+    
+    in_0 <- BSWAP_32 in_0;
+    out <-
+    Array4.init
+    (WArray4.get8 (WArray4.set32_direct (WArray4.init8 (fun i => (out).[i])) 0 (in_0)));
+    return (out);
+  }
+  
   proc __ull_to_bytes_32 (out:W8.t Array32.t, in_0:W64.t) : W8.t Array32.t = {
     var aux: int;
     
@@ -965,13 +976,13 @@ module M(SC:Syscall_t) = {
     return (out);
   }
   
-  proc __ull_to_bytes_2 (out:W8.t Array2.t, in_0:W64.t) : W8.t Array2.t = {
+  proc __ull_to_bytes_4 (out:W8.t Array4.t, in_0:W64.t) : W8.t Array4.t = {
     var aux: int;
     
     var i:int;
     
     aux <- (- 1);
-    i <- (2 - 1);
+    i <- (4 - 1);
     while (aux < i) {
       out.[i] <- (truncateu8 in_0);
       in_0 <- (in_0 `>>` (W8.of_int 8));
@@ -980,13 +991,13 @@ module M(SC:Syscall_t) = {
     return (out);
   }
   
-  proc __ull_to_bytes_4 (out:W8.t Array4.t, in_0:W64.t) : W8.t Array4.t = {
+  proc __ull_to_bytes_2 (out:W8.t Array2.t, in_0:W64.t) : W8.t Array2.t = {
     var aux: int;
     
     var i:int;
     
     aux <- (- 1);
-    i <- (4 - 1);
+    i <- (2 - 1);
     while (aux < i) {
       out.[i] <- (truncateu8 in_0);
       in_0 <- (in_0 `>>` (W8.of_int 8));
@@ -1106,6 +1117,19 @@ module M(SC:Syscall_t) = {
     return (c3);
   }
   
+  proc __memset_zero_u8_4 (a:W8.t Array4.t) : W8.t Array4.t = {
+    
+    var i:W64.t;
+    
+    i <- (W64.of_int 0);
+    
+    while ((i \ult (W64.of_int 4))) {
+      a.[(W64.to_uint i)] <- (W8.of_int 0);
+      i <- (i + (W64.of_int 1));
+    }
+    return (a);
+  }
+  
   proc __memset_u8_4 (a:W8.t Array4.t, value:W8.t) : W8.t Array4.t = {
     
     var i:W64.t;
@@ -1149,14 +1173,14 @@ module M(SC:Syscall_t) = {
     return ();
   }
   
-  proc __memcpy_u8u8_64_64 (out:W8.t Array64.t, offset:W64.t,
-                            in_0:W8.t Array64.t) : W8.t Array64.t * W64.t = {
+  proc __memcpy_u8u8_128_32 (out:W8.t Array128.t, offset:W64.t,
+                             in_0:W8.t Array32.t) : W8.t Array128.t * W64.t = {
     
     var i:W64.t;
     
     i <- (W64.of_int 0);
     
-    while ((i \ult (W64.of_int 64))) {
+    while ((i \ult (W64.of_int 32))) {
       out.[(W64.to_uint offset)] <- in_0.[(W64.to_uint i)];
       i <- (i + (W64.of_int 1));
       offset <- (offset + (W64.of_int 1));
@@ -1179,6 +1203,21 @@ module M(SC:Syscall_t) = {
     return (out, offset);
   }
   
+  proc __memcpy_u8u8_32_32 (out:W8.t Array32.t, offset:W64.t,
+                            in_0:W8.t Array32.t) : W8.t Array32.t * W64.t = {
+    
+    var i:W64.t;
+    
+    i <- (W64.of_int 0);
+    
+    while ((i \ult (W64.of_int 32))) {
+      out.[(W64.to_uint offset)] <- in_0.[(W64.to_uint i)];
+      i <- (i + (W64.of_int 1));
+      offset <- (offset + (W64.of_int 1));
+    }
+    return (out, offset);
+  }
+  
   proc __memcpy_u8u8_64_32 (out:W8.t Array64.t, offset:W64.t,
                             in_0:W8.t Array32.t) : W8.t Array64.t * W64.t = {
     
@@ -1194,14 +1233,14 @@ module M(SC:Syscall_t) = {
     return (out, offset);
   }
   
-  proc __memcpy_u8u8_128_32 (out:W8.t Array128.t, offset:W64.t,
-                             in_0:W8.t Array32.t) : W8.t Array128.t * W64.t = {
+  proc __memcpy_u8u8_64_64 (out:W8.t Array64.t, offset:W64.t,
+                            in_0:W8.t Array64.t) : W8.t Array64.t * W64.t = {
     
     var i:W64.t;
     
     i <- (W64.of_int 0);
     
-    while ((i \ult (W64.of_int 32))) {
+    while ((i \ult (W64.of_int 64))) {
       out.[(W64.to_uint offset)] <- in_0.[(W64.to_uint i)];
       i <- (i + (W64.of_int 1));
       offset <- (offset + (W64.of_int 1));
@@ -1211,21 +1250,6 @@ module M(SC:Syscall_t) = {
   
   proc __memcpy_u8u8_96_32 (out:W8.t Array96.t, offset:W64.t,
                             in_0:W8.t Array32.t) : W8.t Array96.t * W64.t = {
-    
-    var i:W64.t;
-    
-    i <- (W64.of_int 0);
-    
-    while ((i \ult (W64.of_int 32))) {
-      out.[(W64.to_uint offset)] <- in_0.[(W64.to_uint i)];
-      i <- (i + (W64.of_int 1));
-      offset <- (offset + (W64.of_int 1));
-    }
-    return (out, offset);
-  }
-  
-  proc __memcpy_u8u8_32_32 (out:W8.t Array32.t, offset:W64.t,
-                            in_0:W8.t Array32.t) : W8.t Array32.t * W64.t = {
     
     var i:W64.t;
     
@@ -1254,12 +1278,12 @@ module M(SC:Syscall_t) = {
     return (out, offset);
   }
   
-  proc _memcpy_u8u8_64_64 (out:W8.t Array64.t, offset:W64.t,
-                           in_0:W8.t Array64.t) : W8.t Array64.t * W64.t = {
+  proc _memcpy_u8u8_128_32 (out:W8.t Array128.t, offset:W64.t,
+                            in_0:W8.t Array32.t) : W8.t Array128.t * W64.t = {
     
     
     
-    (out, offset) <@ __memcpy_u8u8_64_64 (out, offset, in_0);
+    (out, offset) <@ __memcpy_u8u8_128_32 (out, offset, in_0);
     return (out, offset);
   }
   
@@ -1272,6 +1296,15 @@ module M(SC:Syscall_t) = {
     return (out, offset);
   }
   
+  proc _memcpy_u8u8_32_32 (out:W8.t Array32.t, offset:W64.t,
+                           in_0:W8.t Array32.t) : W8.t Array32.t * W64.t = {
+    
+    
+    
+    (out, offset) <@ __memcpy_u8u8_32_32 (out, offset, in_0);
+    return (out, offset);
+  }
+  
   proc _memcpy_u8u8_64_32 (out:W8.t Array64.t, offset:W64.t,
                            in_0:W8.t Array32.t) : W8.t Array64.t * W64.t = {
     
@@ -1281,12 +1314,12 @@ module M(SC:Syscall_t) = {
     return (out, offset);
   }
   
-  proc _memcpy_u8u8_128_32 (out:W8.t Array128.t, offset:W64.t,
-                            in_0:W8.t Array32.t) : W8.t Array128.t * W64.t = {
+  proc _memcpy_u8u8_64_64 (out:W8.t Array64.t, offset:W64.t,
+                           in_0:W8.t Array64.t) : W8.t Array64.t * W64.t = {
     
     
     
-    (out, offset) <@ __memcpy_u8u8_128_32 (out, offset, in_0);
+    (out, offset) <@ __memcpy_u8u8_64_64 (out, offset, in_0);
     return (out, offset);
   }
   
@@ -1299,24 +1332,15 @@ module M(SC:Syscall_t) = {
     return (out, offset);
   }
   
-  proc _memcpy_u8u8_32_32 (out:W8.t Array32.t, offset:W64.t,
-                           in_0:W8.t Array32.t) : W8.t Array32.t * W64.t = {
-    
-    
-    
-    (out, offset) <@ __memcpy_u8u8_32_32 (out, offset, in_0);
-    return (out, offset);
-  }
-  
-  proc _x_memcpy_u8u8_64_64 (out:W8.t Array64.t, offset:W64.t,
-                             in_0:W8.t Array64.t) : W8.t Array64.t * W64.t = {
+  proc _x_memcpy_u8u8_128_32 (out:W8.t Array128.t, offset:W64.t,
+                              in_0:W8.t Array32.t) : W8.t Array128.t * W64.t = {
     
     
     
     out <- out;
     offset <- offset;
     in_0 <- in_0;
-    (out, offset) <@ _memcpy_u8u8_64_64 (out, offset, in_0);
+    (out, offset) <@ _memcpy_u8u8_128_32 (out, offset, in_0);
     out <- out;
     offset <- offset;
     return (out, offset);
@@ -1336,6 +1360,20 @@ module M(SC:Syscall_t) = {
     return (out, offset);
   }
   
+  proc _x_memcpy_u8u8_32_32 (out:W8.t Array32.t, offset:W64.t,
+                             in_0:W8.t Array32.t) : W8.t Array32.t * W64.t = {
+    
+    
+    
+    out <- out;
+    offset <- offset;
+    in_0 <- in_0;
+    (out, offset) <@ _memcpy_u8u8_32_32 (out, offset, in_0);
+    out <- out;
+    offset <- offset;
+    return (out, offset);
+  }
+  
   proc _x_memcpy_u8u8_64_32 (out:W8.t Array64.t, offset:W64.t,
                              in_0:W8.t Array32.t) : W8.t Array64.t * W64.t = {
     
@@ -1350,15 +1388,15 @@ module M(SC:Syscall_t) = {
     return (out, offset);
   }
   
-  proc _x_memcpy_u8u8_128_32 (out:W8.t Array128.t, offset:W64.t,
-                              in_0:W8.t Array32.t) : W8.t Array128.t * W64.t = {
+  proc _x_memcpy_u8u8_64_64 (out:W8.t Array64.t, offset:W64.t,
+                             in_0:W8.t Array64.t) : W8.t Array64.t * W64.t = {
     
     
     
     out <- out;
     offset <- offset;
     in_0 <- in_0;
-    (out, offset) <@ _memcpy_u8u8_128_32 (out, offset, in_0);
+    (out, offset) <@ _memcpy_u8u8_64_64 (out, offset, in_0);
     out <- out;
     offset <- offset;
     return (out, offset);
@@ -1378,17 +1416,19 @@ module M(SC:Syscall_t) = {
     return (out, offset);
   }
   
-  proc _x_memcpy_u8u8_32_32 (out:W8.t Array32.t, offset:W64.t,
-                             in_0:W8.t Array32.t) : W8.t Array32.t * W64.t = {
+  proc __memcpy_u8u8p_32 (out:W8.t Array32.t, offset:W64.t, in_0:W64.t,
+                          inlen:W64.t) : W8.t Array32.t * W64.t = {
     
+    var i:W64.t;
     
+    i <- (W64.of_int 0);
     
-    out <- out;
-    offset <- offset;
-    in_0 <- in_0;
-    (out, offset) <@ _memcpy_u8u8_32_32 (out, offset, in_0);
-    out <- out;
-    offset <- offset;
+    while ((i \ult inlen)) {
+      out.[(W64.to_uint offset)] <-
+      (loadW8 Glob.mem (W64.to_uint (in_0 + i)));
+      i <- (i + (W64.of_int 1));
+      offset <- (offset + (W64.of_int 1));
+    }
     return (out, offset);
   }
   
@@ -1408,31 +1448,6 @@ module M(SC:Syscall_t) = {
     return (out, offset);
   }
   
-  proc __memcpy_u8u8p_32 (out:W8.t Array32.t, offset:W64.t, in_0:W64.t,
-                          inlen:W64.t) : W8.t Array32.t * W64.t = {
-    
-    var i:W64.t;
-    
-    i <- (W64.of_int 0);
-    
-    while ((i \ult inlen)) {
-      out.[(W64.to_uint offset)] <-
-      (loadW8 Glob.mem (W64.to_uint (in_0 + i)));
-      i <- (i + (W64.of_int 1));
-      offset <- (offset + (W64.of_int 1));
-    }
-    return (out, offset);
-  }
-  
-  proc _memcpy_u8u8p_64 (out:W8.t Array64.t, offset:W64.t, in_0:W64.t,
-                         inlen:W64.t) : W8.t Array64.t * W64.t = {
-    
-    
-    
-    (out, offset) <@ __memcpy_u8u8p_64 (out, offset, in_0, inlen);
-    return (out, offset);
-  }
-  
   proc _memcpy_u8u8p_32 (out:W8.t Array32.t, offset:W64.t, in_0:W64.t,
                          inlen:W64.t) : W8.t Array32.t * W64.t = {
     
@@ -1442,17 +1457,12 @@ module M(SC:Syscall_t) = {
     return (out, offset);
   }
   
-  proc _x_memcpy_u8u8p_64 (out:W8.t Array64.t, offset:W64.t, in_0:W64.t,
-                           inlen:W64.t) : W8.t Array64.t * W64.t = {
+  proc _memcpy_u8u8p_64 (out:W8.t Array64.t, offset:W64.t, in_0:W64.t,
+                         inlen:W64.t) : W8.t Array64.t * W64.t = {
     
     
     
-    out <- out;
-    offset <- offset;
-    in_0 <- in_0;
-    (out, offset) <@ _memcpy_u8u8p_64 (out, offset, in_0, inlen);
-    out <- out;
-    offset <- offset;
+    (out, offset) <@ __memcpy_u8u8p_64 (out, offset, in_0, inlen);
     return (out, offset);
   }
   
@@ -1470,9 +1480,23 @@ module M(SC:Syscall_t) = {
     return (out, offset);
   }
   
-  proc __memcpy_u8u8_2_64_2144 (out:W8.t Array64.t, out_offset:W64.t,
+  proc _x_memcpy_u8u8p_64 (out:W8.t Array64.t, offset:W64.t, in_0:W64.t,
+                           inlen:W64.t) : W8.t Array64.t * W64.t = {
+    
+    
+    
+    out <- out;
+    offset <- offset;
+    in_0 <- in_0;
+    (out, offset) <@ _memcpy_u8u8p_64 (out, offset, in_0, inlen);
+    out <- out;
+    offset <- offset;
+    return (out, offset);
+  }
+  
+  proc __memcpy_u8u8_2_32_2144 (out:W8.t Array32.t, out_offset:W64.t,
                                 in_0:W8.t Array2144.t, in_offset:W64.t,
-                                bytes:W64.t) : W8.t Array64.t * W64.t * W64.t = {
+                                bytes:W64.t) : W8.t Array32.t * W64.t * W64.t = {
     
     var i:W64.t;
     
@@ -1487,9 +1511,9 @@ module M(SC:Syscall_t) = {
     return (out, out_offset, in_offset);
   }
   
-  proc __memcpy_u8u8_2_32_2144 (out:W8.t Array32.t, out_offset:W64.t,
+  proc __memcpy_u8u8_2_64_2144 (out:W8.t Array64.t, out_offset:W64.t,
                                 in_0:W8.t Array2144.t, in_offset:W64.t,
-                                bytes:W64.t) : W8.t Array32.t * W64.t * W64.t = {
+                                bytes:W64.t) : W8.t Array64.t * W64.t * W64.t = {
     
     var i:W64.t;
     
@@ -1756,14 +1780,12 @@ module M(SC:Syscall_t) = {
     var aux: int;
     
     var i:int;
-    var t:W64.t;
     var buf:W8.t Array4.t;
     buf <- witness;
     i <- 0;
     while (i < 8) {
-      t <- (zeroextu64 addr.[i]);
       buf <- (Array4.init (fun i_0 => addr_as_bytes.[(4 * i) + i_0]));
-      buf <@ __ull_to_bytes_4 (buf, t);
+      buf <@ __u32_to_bytes (buf, addr.[i]);
       addr_as_bytes <- Array32.init
                        (fun i_0 => if (4 * i) <= i_0 < (4 * i) + 4
                        then buf.[i_0-(4 * i)] else addr_as_bytes.[i_0]);
@@ -2268,45 +2290,6 @@ module M(SC:Syscall_t) = {
     return (out, addr);
   }
   
-  proc __base_w_3_2 (output:W32.t Array3.t, input:W8.t Array2.t) : W32.t Array3.t = {
-    
-    var in_0:W64.t;
-    var out:W64.t;
-    var bits:W64.t;
-    var consumed:W64.t;
-    var total:W8.t;
-    var total_32:W32.t;
-    var _of_:bool;
-    var _cf_:bool;
-    var _sf_:bool;
-    var _zf_:bool;
-    var  _0:bool;
-    
-    in_0 <- (W64.of_int 0);
-    out <- (W64.of_int 0);
-    bits <- (W64.of_int 0);
-    consumed <- (W64.of_int 0);
-    
-    while ((consumed \ult (W64.of_int 3))) {
-      if ((bits = (W64.of_int 0))) {
-        total <- input.[(W64.to_uint in_0)];
-        in_0 <- (in_0 + (W64.of_int 1));
-        bits <- (bits + (W64.of_int 8));
-      } else {
-        
-      }
-      bits <- (bits - (W64.of_int 4));
-      total_32 <- (zeroextu32 total);
-      (_of_, _cf_, _sf_,  _0, _zf_, total_32) <- SHR_32 total_32
-      (truncateu8 bits);
-      total_32 <- (total_32 `&` (W32.of_int (16 - 1)));
-      output.[(W64.to_uint out)] <- total_32;
-      out <- (out + (W64.of_int 1));
-      consumed <- (consumed + (W64.of_int 1));
-    }
-    return (output);
-  }
-  
   proc __base_w_67_32 (output:W32.t Array67.t, input:W8.t Array32.t) : 
   W32.t Array67.t = {
     
@@ -2328,6 +2311,45 @@ module M(SC:Syscall_t) = {
     consumed <- (W64.of_int 0);
     
     while ((consumed \ult (W64.of_int 67))) {
+      if ((bits = (W64.of_int 0))) {
+        total <- input.[(W64.to_uint in_0)];
+        in_0 <- (in_0 + (W64.of_int 1));
+        bits <- (bits + (W64.of_int 8));
+      } else {
+        
+      }
+      bits <- (bits - (W64.of_int 4));
+      total_32 <- (zeroextu32 total);
+      (_of_, _cf_, _sf_,  _0, _zf_, total_32) <- SHR_32 total_32
+      (truncateu8 bits);
+      total_32 <- (total_32 `&` (W32.of_int (16 - 1)));
+      output.[(W64.to_uint out)] <- total_32;
+      out <- (out + (W64.of_int 1));
+      consumed <- (consumed + (W64.of_int 1));
+    }
+    return (output);
+  }
+  
+  proc __base_w_3_2 (output:W32.t Array3.t, input:W8.t Array2.t) : W32.t Array3.t = {
+    
+    var in_0:W64.t;
+    var out:W64.t;
+    var bits:W64.t;
+    var consumed:W64.t;
+    var total:W8.t;
+    var total_32:W32.t;
+    var _of_:bool;
+    var _cf_:bool;
+    var _sf_:bool;
+    var _zf_:bool;
+    var  _0:bool;
+    
+    in_0 <- (W64.of_int 0);
+    out <- (W64.of_int 0);
+    bits <- (W64.of_int 0);
+    consumed <- (W64.of_int 0);
+    
+    while ((consumed \ult (W64.of_int 3))) {
       if ((bits = (W64.of_int 0))) {
         total <- input.[(W64.to_uint in_0)];
         in_0 <- (in_0 + (W64.of_int 1));
@@ -3364,8 +3386,7 @@ module M(SC:Syscall_t) = {
     top_tree_addr <- witness;
     top_tree_addr <@ __zero_address (top_tree_addr);
     top_tree_addr <@ __set_layer_addr (top_tree_addr, (W32.of_int (1 - 1)));
-    aux <@ __memset_u8_4 ((Array4.init (fun i_0 => sk.[0 + i_0])),
-    (W8.of_int 0));
+    aux <@ __memset_zero_u8_4 ((Array4.init (fun i_0 => sk.[0 + i_0])));
     sk <- Array132.init
           (fun i_0 => if 0 <= i_0 < 0 + 4 then aux.[i_0-0] else sk.[i_0]);
     (aux_0,
